x86/RelocBingenproofArchi.v
@@ -2,7 +2,7 @@ Require Import Coqlib Maps AST lib.Integers Values.
 Require Import Events lib.Floats Memory Smallstep.
 Require Import Asm RelocProg RelocProgramBytes.
 Require Import Stacklayout Conventions.
-Require Import Linking RelocProgLinking Errors.
+Require Import Linking RelocProgLinking Errors.   
 Require Import EncDecRet RelocBingen RelocBinDecode.
 Require Import RelocProgSemantics RelocProgSemantics1.
 Require Import TranslateInstr RelocProgSemantics2.
